Improve while loop idiom, start cleaning up

src/Enumeration/Loopers.dfy
@@ -225,106 +225,6 @@ module Loopers {
     }
   }
 
-  iterator SeqIterator<T(0)>(s: seq<T>) yields (element: T)
-    yield ensures elements <= s
-    ensures elements == s
-  {
-    for i := 0 to |s|
-      invariant i == |elements|
-      invariant elements <= s
-    {
-      yield s[i];
-    }
-  }
-
-  class SeqIteratorEnumerator<T(0)> extends Enumerator<T> {
-
-    const iter: SeqIterator<T>
-    var done: bool
-
-    ghost const original: seq<T>
-
-    constructor(s: seq<T>) 
-      ensures Valid() 
-      ensures fresh(Repr) 
-    {
-      iter := new SeqIterator(s);
-      original := s;
-      enumerated := [];
-      
-      new;
-
-      // Calling MoveNext() right away ensures we only enumerated yielded state.
-      // Another version of this adaptor could not do this, and by consequence
-      // enumerate the initial state of the iterator as well.
-      var more := iter.MoveNext();
-      done := !more;
-      
-      Repr := {this, iter} + iter._modifies + iter._reads + iter._new;
-    }
-
-    predicate Valid() reads this, Repr ensures Valid() ==> this in Repr {
-      && this in Repr
-      && iter in Repr
-      && this !in iter._modifies
-      && this !in iter._reads
-      && this !in iter._new
-      && iter._modifies <= Repr
-      && iter._reads <= Repr
-      && iter._new <= Repr
-      && (!done ==> iter.Valid())
-      && (!done ==> enumerated + [Current()] == iter.elements)
-      && (done ==> enumerated == iter.elements)
-      && iter.elements < iter.s
-      && |enumerated| <= |original|
-      && enumerated == original[0..|enumerated|]
-    } 
-
-    predicate method Done()
-      requires Valid()
-      reads this, Repr
-      decreases Repr, 0
-      ensures Decreases() == 0 ==> Done()
-      // ensures Done() ==> enumerated == original
-    {
-      done
-    }
-
-    method Step()
-      requires Valid()
-      requires !Done()
-      modifies Repr
-      decreases Repr
-      ensures Valid()
-      ensures Repr <= old(Repr) 
-      ensures Decreases() < old(Decreases())
-      ensures enumerated == old(enumerated) + [old(Current())]
-    {
-      enumerated := enumerated + [Current()];
-
-      var more := iter.MoveNext();
-      done := !more;
-
-      Repr := {this, iter} + iter._modifies + iter._reads + iter._new;
-    }
-
-    function method Current(): T
-      reads this, Repr
-      requires Valid()
-      requires !Done()
-    {
-      iter.element
-    }
-
-    function Decreases(): nat 
-      reads this, Repr 
-      requires Valid() 
-    {
-      assert iter.elements < iter.s;
-      (|iter.s| - |iter.elements|) //+ (if done then 0 else 1)
-    }
-  }
-
   class ConcatEnumerator<T(0)> extends Enumerator<T> {
 
     const first: Enumerator<T>
@@ -339,8 +239,8 @@ module Loopers {
     {
       this.first := first;
       this.second := second;
-      enumerated := [];
       
+      enumerated := [];
       Repr := {this} + first.Repr + second.Repr;
     }
 
@@ -470,13 +370,12 @@ module Loopers {
   method Example1() {
     var numbers := [1, 2, 3, 4, 5];
     var e: Enumerator<int> := new SeqEnumerator(numbers);
-    label start:
     while (!e.Done()) 
-      invariant e.Valid()
-      invariant old@start(allocated(e)) && fresh(e.Repr)
+      invariant e.Valid() && fresh(e.Repr)
       decreases e.Decreases()
     {
       print e.Current(), "\n";
+
       e.Step();
     }
   }
@@ -485,13 +384,12 @@ module Loopers {
     var maybeNumbers := [Some(1), Some(2), Some(3), None, None];
     var e: Enumerator<Option<int>> := new SeqEnumerator(maybeNumbers);
     var e': Enumerator<int> := new TerminatedEnumerator(e);
-    label start:
     while (!e'.Done()) 
-      invariant e'.Valid()
-      invariant old@start(allocated(e')) && fresh(e'.Repr)
+      invariant e'.Valid() && fresh(e'.Repr)
       decreases e'.Decreases()
     {
       print e'.Current(), "\n";
+
       e'.Step();
     }
   }
@@ -503,10 +401,8 @@ module Loopers {
     var e2 := new SeqEnumerator(second);
     var e := new ConcatEnumerator(e1, e2);
    
-    label start:
     while (!e.Done()) 
-      invariant e.Valid()
-      invariant fresh(e.Repr)
+      invariant e.Valid() && fresh(e.Repr)
       decreases e.Decreases()
     {
       print e.Current(), "\n";
