src/Enumeration/IteratorAdaptor.dfy
@@ -1,0 +1,121 @@
+
+include "Loopers.dfy"
+
+module IteratorAdaptorExample {
+
+  import opened Loopers
+
+  iterator SeqIterator<T(0)>(s: seq<T>) yields (element: T)
+    yield ensures elements <= s
+    ensures elements == s
+  {
+    for i := 0 to |s|
+      invariant i == |elements|
+      invariant elements <= s
+    {
+      yield s[i];
+    }
+  }
+
+  class SeqIteratorEnumerator<T(0)> extends Enumerator<T> {
+
+    const iter: SeqIterator<T>
+    var done: bool
+
+    ghost const original: seq<T>
+    ghost var decr: nat
+
+    constructor(s: seq<T>) 
+      ensures Valid() 
+      ensures fresh(Repr) 
+    {
+      iter := new SeqIterator(s);
+      original := s;
+      enumerated := [];
+      
+      new;
+
+      // Calling MoveNext() right away ensures we only enumerate yielded state.
+      var more := iter.MoveNext();
+      done := !more;
+      
+      Repr := {this, iter} + iter._modifies + iter._reads + iter._new;
+      decr := |iter.s| - |enumerated|;
+      assert !done ==> iter.elements < iter.s; 
+    }
+
+    predicate Valid() reads this, Repr ensures Valid() ==> this in Repr {
+      && this in Repr
+      && iter in Repr
+      && this !in iter._modifies
+      && this !in iter._reads
+      && this !in iter._new
+      && iter._modifies <= Repr
+      && iter._reads <= Repr
+      && iter._new <= Repr
+      && (!done ==> iter.Valid())
+      && (!done ==> enumerated + [iter.element] == iter.elements)
+      && (done ==> enumerated == iter.elements)
+      && (!done ==> iter.elements < iter.s)
+      && decr == |iter.s| - |enumerated|
+    } 
+
+    predicate method Done()
+      requires Valid()
+      reads this, Repr
+      decreases Repr, 0
+      ensures Decreases() == 0 ==> Done()
+    {
+      done
+    }
+
+    method Step()
+      requires Valid()
+      requires !Done()
+      modifies Repr
+      decreases Repr
+      ensures Valid()
+      ensures Repr <= old(Repr) 
+      ensures Decreases() < old(Decreases())
+      ensures enumerated == old(enumerated) + [old(Current())]
+    {
+      enumerated := enumerated + [Current()];
+
+      var more := iter.MoveNext();
+      done := !more;
+      
+      assert iter._new == {};
+
+      Repr := {this, iter} + iter._modifies + iter._reads + iter._new;
+      decr := |iter.s| - |enumerated|;
+
+      assert this in Repr;
+      assert iter in Repr;
+      assert this !in iter._modifies;
+      assert this !in iter._reads;
+      assert this !in iter._new;
+      assert iter._modifies <= Repr;
+      assert iter._reads <= Repr;
+      assert iter._new <= Repr;
+      assert (!done ==> iter.Valid());
+      assert (!done ==> enumerated + [iter.element] == iter.elements);
+      assert (done ==> enumerated == iter.elements);
+      assert !done ==> iter.elements < iter.s; 
+    }
+
+    function method Current(): T
+      reads this, Repr
+      requires Valid()
+      requires !Done()
+    {
+      iter.element
+    }
+
+    function Decreases(): nat 
+      reads this, Repr 
+      requires Valid() 
+    {
+      decr
+    }
+  }
+}
